Added an injection universe, so that local variables can have different types.

UTP/ITree_Local_Var.thy
@@ -2,21 +2,87 @@ theory ITree_Local_Var
   imports ITree_Hoare
 begin
 
+datatype utype =
+  UnitT | BoolT | NatT | IntT | RatT | RealT | StringT | ListT utype | PairT utype utype | SumT utype utype
+
+datatype uval =
+  UnitV | BoolV bool | NatV nat | IntV int | RatV rat | RealV real | StringV "String.literal" | 
+  ListV utype "uval list" | PairV "uval \<times> uval" | SumV utype utype "uval + uval"
+
+fun uval_type :: "uval \<Rightarrow> utype option" where
+"uval_type UnitV = Some UnitT" |
+"uval_type (BoolV _) = Some BoolT" |
+"uval_type (NatV _) = Some NatT" |
+"uval_type (IntV _) = Some IntT" | 
+"uval_type (RatV _) = Some RatT" |
+"uval_type (RealV _) = Some RealT" |
+"uval_type (StringV _) = Some StringT" |
+"uval_type (ListV t xs) = (if (\<forall> x\<in>set xs. uval_type x = Some t) then Some (ListT t) else None)" |
+"uval_type (PairV (x, y)) = (case (uval_type x, uval_type y) of (Some a, Some b) \<Rightarrow> Some (PairT a b) | _ \<Rightarrow> None)" |
+"uval_type (SumV a b x) = (if (case x of Inl l \<Rightarrow> uval_type l = Some a | Inr r \<Rightarrow> uval_type r = Some b) then Some (SumT a b) else None)" 
+
+class injval =
+  fixes inj_val :: "'a \<Rightarrow> uval"
+  and proj_val :: "uval \<Rightarrow> 'a option"
+  and utyp :: "'a itself \<Rightarrow> utype"
+  assumes inj_val_inv [simp]: "proj_val (inj_val x) = Some x"
+  and val_type [simp]: "uval_type (inj_val x) = Some (utyp TYPE('a))" 
+
+instantiation bool :: injval
+begin
+definition inj_val_bool :: "bool \<Rightarrow> uval" where "inj_val_bool = BoolV"
+fun proj_val_bool :: "uval \<Rightarrow> bool option" where "proj_val x = (case x of BoolV n \<Rightarrow> Some n | _ \<Rightarrow> None)"
+definition utyp_bool :: "bool itself \<Rightarrow> utype" where "utyp_bool t = BoolT"
+instance by (intro_classes, auto simp add: inj_val_bool_def utyp_bool_def)
+end
+
+instantiation nat :: injval
+begin
+definition inj_val_nat :: "nat \<Rightarrow> uval" where "inj_val_nat = NatV"
+fun proj_val_nat :: "uval \<Rightarrow> nat option" where "proj_val x = (case x of NatV n \<Rightarrow> Some n | _ \<Rightarrow> None)"
+definition utyp_nat :: "nat itself \<Rightarrow> utype" where "utyp_nat t = NatT"
+instance by (intro_classes, auto simp add: inj_val_nat_def utyp_nat_def)
+end
+
+instantiation int :: injval
+begin
+definition inj_val_int :: "int \<Rightarrow> uval" where "inj_val_int = IntV"
+fun proj_val_int :: "uval \<Rightarrow> int option" where "proj_val x = (case x of IntV n \<Rightarrow> Some n | _ \<Rightarrow> None)"
+definition utyp_int :: "int itself \<Rightarrow> utype" where "utyp_int t = IntT"
+instance by (intro_classes, auto simp add: inj_val_int_def utyp_int_def)
+end
+
+instantiation list :: (injval) injval
+begin
+definition inj_val_list :: "'a list \<Rightarrow> uval" where "inj_val_list xs = ListV (utyp TYPE('a)) (map inj_val xs)"
+definition proj_val_list :: "uval \<Rightarrow> 'a list option" 
+  where "proj_val x = (case x of ListV a xs \<Rightarrow> let ys = map proj_val xs in (if None \<in> set ys then None else Some (map the ys)) |
+                                 _ \<Rightarrow> None)"
+definition utyp_list :: "'a list itself \<Rightarrow> utype" where "utyp_list t = ListT (utyp TYPE('a))"
+instance by (intro_classes, auto simp add: inj_val_list_def proj_val_list_def utyp_list_def list.map_ident_strong)
+end
+
+definition uval_lens :: "'a::injval \<Longrightarrow> uval" where
+"uval_lens = \<lparr> lens_get = (\<lambda> s. the (proj_val s)), lens_put = (\<lambda> s v. inj_val v) \<rparr>"  
+
+lemma mwb_uval_lens [simp]: "mwb_lens uval_lens"
+  by (unfold_locales, simp_all add: uval_lens_def)
+
 zstore lvar =
-  lstack :: "int list"
+  lstack :: "uval list"
 
 definition open_var :: "('e, 'a lvar_scheme) htree" where
-"open_var = (lstack := lstack @ [0])"
+"open_var = (lstack := lstack @ [UnitV])"
 
 definition close_var :: "('e, 'a lvar_scheme) htree" where
 "close_var = (lstack := butlast lstack)"
 
-definition "lvar_lens l = (list_lens (length l - 1) ;\<^sub>L lstack)"
+definition "lvar_lens l = (uval_lens ;\<^sub>L list_lens (length l - 1) ;\<^sub>L lstack)"
 
 lemma mwb_lvar_lens [simp]: "mwb_lens (lvar_lens s)"
   by (simp add: lvar_lens_def list_mwb_lens comp_mwb_lens)
 
-definition vblock :: "((int \<Longrightarrow> 'a lvar_scheme) \<Rightarrow> ('e, 'a lvar_scheme) htree) \<Rightarrow> ('e, 'a lvar_scheme) htree"
+definition vblock :: "(('v::injval \<Longrightarrow> 'a lvar_scheme) \<Rightarrow> ('e, 'a lvar_scheme) htree) \<Rightarrow> ('e, 'a lvar_scheme) htree"
   where "vblock B = open_var ;; let_itree (SEXP (\<lambda> s. (lvar_lens (get\<^bsub>lstack\<^esub> s)))) B ;; close_var"
 
 syntax "_vblock" :: "id \<Rightarrow> type \<Rightarrow> logic \<Rightarrow> logic" ("var _ :: _./ _" [0, 0, 10] 10)
@@ -25,7 +91,7 @@ translations
   "_vblock x t e" => "CONST vblock (_lvar_abs x t e)"
 
 definition "lv_at x n = (\<lambda> s. length (get\<^bsub>lstack\<^esub> s) > n 
-                        \<and> x = list_lens (length (get\<^bsub>lstack\<^esub> s) - Suc n) ;\<^sub>L lstack)"
+                        \<and> x = uval_lens ;\<^sub>L list_lens (length (get\<^bsub>lstack\<^esub> s) - Suc n) ;\<^sub>L lstack)"
 
 expr_constructor lv_at
 
@@ -37,8 +103,8 @@ lemma lv_at_indep_out_stack2 [simp]: "\<lbrakk> lv_at x n s; lstack \<bowtie> y 
 
 lemma lv_at_indep_in_stack [simp]: "\<lbrakk> lv_at x m s; lv_at y n s; m \<noteq> n \<rbrakk> \<Longrightarrow> x \<bowtie> y"
   by (simp add: lv_at_def lens_comp_indep_cong)
-     (metis cancel_semigroup_add_class.add_left_imp_eq diff_diff_cancel less_eq_Suc_le list_lens_indep plus_1_eq_Suc)
-
+     (metis Suc_diff_Suc diff_less_mono2 lens_indep_left_ext lens_indep_right_ext list_lens_indep nat_neq_iff)
+     
 lemma lv_at_grow_stack_1 [usubst]: "(lv_at x n)\<lbrakk>butlast lstack/lstack\<rbrakk> = lv_at x (n + 1)"
   by (auto simp add: lv_at_def subst_app_def subst_upd_def fun_eq_iff)
 
@@ -69,7 +135,7 @@ zstore swap = lvar +
 lit_vars
 
 definition prog :: "(unit, swap) htree" where 
-"prog = (var temp2::int. var temp::int. temp := x ;; x := y ;; y := temp)"
+"prog = (var temp2::nat list. var temp::int. temp := x ;; x := y ;; y := temp)"
 
 lemma "H{x = X \<and> y = Y} prog {x = Y \<and> y = X}"
   unfolding prog_def
